system and spec

messageInvariantPrototypes/lib/UtilitiesLibrary.dfy
@@ -163,6 +163,11 @@ module UtilitiesLibrary {
     m'
   }
 
+  ghost predicate IsSeqExtension<T>(s: seq<T>, s': seq<T>) {
+    && |s'| == |s| + 1
+    && forall i | 0 <= i < |s| :: s[i] == s'[i]
+  }
+
   ghost function StutterSeq<T>(s: seq<T>) : (s': seq<T>)
     requires 0 < |s|
     ensures |s'| == |s|+1
