messageInvariantPrototypes/paxos/centralizedMonotonic_globalHistory/system.dfy
@@ -1,0 +1,257 @@
+include "hosts.dfy"
+
+module System {
+  import opened UtilitiesLibrary
+  import opened Types
+  import LeaderHost
+  import AcceptorHost
+  import LearnerHost
+
+datatype Constants = Constants(
+  f: nat,
+  leaderConstants: seq<LeaderHost.Constants>,
+  acceptorConstants: seq<AcceptorHost.Constants>,
+  learnerConstants: seq<LearnerHost.Constants>
+)
+{
+  ghost predicate WF() {
+    && 0 < f
+    && UniqueIds()
+  }
+  
+  ghost predicate UniqueIds() {
+    && UniqueLeaderIds()
+    && UniqueAcceptorIds()
+    && UniqueLearnerIds()
+  }
+
+  ghost predicate ValidLeaderIdx(id: int) {
+    0 <= id < |leaderConstants|
+  }
+
+  ghost predicate ValidAcceptorIdx(id: int) {
+    0 <= id < |acceptorConstants|
+  }
+
+  ghost predicate ValidLearnerIdx(id: int) {
+    0 <= id < |learnerConstants|
+  }
+  
+  ghost predicate UniqueLeaderIds() {
+    forall i, j | ValidLeaderIdx(i) && ValidLeaderIdx(j) && leaderConstants[i].id == leaderConstants[j].id :: i == j
+  }
+
+  ghost predicate UniqueAcceptorIds() {
+    forall i, j | ValidAcceptorIdx(i) && ValidAcceptorIdx(j) && acceptorConstants[i].id == acceptorConstants[j].id :: i == j
+  }
+
+  ghost predicate UniqueLearnerIds() {
+    forall i, j | ValidLearnerIdx(i) && ValidLearnerIdx(j) && learnerConstants[i].id == learnerConstants[j].id :: i == j
+  }
+} // end datatype Constants
+
+datatype Hosts = Hosts(
+  leaders: seq<LeaderHost.Variables>,
+  acceptors: seq<AcceptorHost.Variables>,
+  learners: seq<LearnerHost.Variables>
+) {
+  ghost predicate WF(c: Constants) {
+    && LeaderHost.GroupWF(c.leaderConstants, leaders, c.f)
+    && AcceptorHost.GroupWF(c.acceptorConstants, acceptors, c.f)
+    && LearnerHost.GroupWF(c.learnerConstants, learners, c.f)
+  }
+
+  ghost predicate LeaderCanPropose(c: Constants, ldr: LeaderId) 
+    requires WF(c)
+    requires c.ValidLeaderIdx(ldr)
+  {
+    leaders[ldr].CanPropose(c.leaderConstants[ldr])
+  }
+}
+
+datatype Variables = Variables(
+  history: seq<Hosts>
+)
+{
+  ghost predicate ValidHistoryIdx(i: int) {
+    0 <= i < |history|
+  }
+
+  ghost predicate WF(c: Constants) {
+    && c.WF()
+    && 0 < |history|
+    && (forall i | ValidHistoryIdx(i) :: history[i].WF(c))
+  }
+
+  ghost function Last() : Hosts 
+    requires 0 < |history|
+  {
+    UtilitiesLibrary.Last(history)
+  }
+} // end datatype Variables
+
+
+//// System Transitions ////
+
+ghost predicate Init(c: Constants, v: Variables) {
+  && v.WF(c)
+  && |v.history| == 1
+  && LeaderHost.GroupInit(c.leaderConstants, v.history[0].leaders, c.f)
+  && AcceptorHost.GroupInit(c.acceptorConstants, v.history[0].acceptors, c.f)
+  && LearnerHost.GroupInit(c.learnerConstants, v.history[0].learners, c.f)
+}
+
+datatype Step = 
+  | P1aStep(leader: LeaderId, acceptor: AcceptorId)
+  | P1bStep(acceptor: AcceptorId, leader: LeaderId, balOpt:Option<LeaderId>, vbOptOpt:Option<Option<ValBal>>)
+  | P2aStep(leader: LeaderId, acceptor: AcceptorId, val: Value)
+  | P2bStep(acceptor: AcceptorId, learner: LearnerId, acceptedVb: ValBal)
+  | LearnerInternalStep(learner: LearnerId)
+  | StutterStep()
+
+
+// Leader sends Prepare message to Acceptor. Acceptor buffers it in its pendingPrepare field 
+ghost predicate NextP1aStep(c: Constants, v: Variables, v': Variables, ldr: LeaderId, acc: AcceptorId) 
+  requires v.WF(c) && v'.WF(c)
+{
+  var ldrLbl := LeaderHost.PrepareLbl();
+  var accLbl := AcceptorHost.ReceivePrepareLbl(ldr);
+  && c.ValidLeaderIdx(ldr)
+  && c.ValidAcceptorIdx(acc)
+  && IsSeqExtension(v.history, v'.history)
+  && AcceptorHost.Next(c.acceptorConstants[acc], v.Last().acceptors[acc], v'.Last().acceptors[acc], accLbl)
+  && AcceptorsUnchangedExcept(c, v.Last(), v'.Last(), acc)
+  && LeaderHost.Next(c.leaderConstants[ldr], v.Last().leaders[ldr], v'.Last().leaders[ldr], ldrLbl)
+  && LeadersUnchangedExcept(c, v.Last(), v'.Last(), ldr)
+  && LearnersUnchanged(v.Last(), v'.Last())
+}
+
+// Acceptor processes its pendingPrepare, and maybe sends a Promise to the leader
+ghost predicate NextP1bStep(c: Constants, v: Variables, v': Variables, 
+    ldr: LeaderId, acc: AcceptorId,
+    balOpt: Option<LeaderId>, vbOptOpt: Option<Option<ValBal>>) 
+  requires v.WF(c) && v'.WF(c)
+{
+  var accLbl := AcceptorHost.MaybePromiseLbl(balOpt, vbOptOpt);
+  && c.ValidLeaderIdx(ldr)
+  && c.ValidAcceptorIdx(acc)
+  && AcceptorHost.Next(c.acceptorConstants[acc], v.Last().acceptors[acc], v'.Last().acceptors[acc], accLbl)
+  && AcceptorsUnchangedExcept(c, v.Last(), v'.Last(), acc)
+  && LearnersUnchanged(v.Last(), v'.Last())
+  && if balOpt.Some? then
+        // assert vbOptOpt.Some?;
+        && var ldrLbl := LeaderHost.ReceivePromiseLbl(acc, vbOptOpt.value);
+        && ldr == balOpt.value
+        && LeaderHost.Next(c.leaderConstants[ldr], v.Last().leaders[ldr], v'.Last().leaders[ldr], ldrLbl)
+        && LeadersUnchangedExcept(c, v.Last(), v'.Last(), ldr)
+      else 
+        LeadersUnchanged(v.Last(), v'.Last())
+}
+
+// Leader sends Proposal to an acceptor. The acceptor processes the proposal
+ghost predicate NextP2aStep(c: Constants, v: Variables, v': Variables, 
+    ldr: LeaderId, acc: AcceptorId,
+    val: Value) 
+  requires v.WF(c) && v'.WF(c)
+{
+  var ldrLbl := LeaderHost.ProposeLbl(val);
+  var accLbl := AcceptorHost.MaybeAcceptLbl(ldr, val);
+  && c.ValidLeaderIdx(ldr)
+  && c.ValidAcceptorIdx(acc)
+  && LeaderHost.Next(c.leaderConstants[ldr], v.Last().leaders[ldr], v'.Last().leaders[ldr], ldrLbl)
+  && AcceptorHost.Next(c.acceptorConstants[acc], v.Last().acceptors[acc], v'.Last().acceptors[acc], accLbl)
+  && LeadersUnchangedExcept(c, v.Last(), v'.Last(), ldr)
+  && AcceptorsUnchangedExcept(c, v.Last(), v'.Last(), acc)
+  && LearnersUnchanged(v.Last(), v'.Last())
+}
+
+// Acceptor sends acceptedVB to some Learner
+ghost predicate NextP2bStep(c: Constants, v: Variables, v': Variables, 
+    acc: AcceptorId, lnr: LearnerId,
+    acceptedVb: ValBal)
+  requires v.WF(c) && v'.WF(c)
+{
+  var accLbl := AcceptorHost.BroadcastAcceptedLbl(acceptedVb);
+  var lnrLbl := LearnerHost.ReceiveAcceptLbl(acceptedVb, acc);
+  && c.ValidAcceptorIdx(acc)
+  && c.ValidLearnerIdx(lnr)
+  // acceptor simply stutters
+  && AcceptorHost.Next(c.acceptorConstants[acc], v.Last().acceptors[acc], v'.Last().acceptors[acc], accLbl)
+  && AcceptorsUnchangedExcept(c, v.Last(), v'.Last(), acc)
+  && LeadersUnchanged(v.Last(), v'.Last())
+  // learner receives accepted vb from acceptor
+  && LearnerHost.Next(c.learnerConstants[lnr], v.Last().learners[lnr], v'.Last().learners[lnr], lnrLbl)
+  && LearnersUnchangedExcept(c, v.Last(), v'.Last(), lnr)
+}
+
+ghost predicate NextLearnerInternalStep(c: Constants, v: Variables, v': Variables, lnr: LearnerId)
+  requires v.WF(c) && v'.WF(c)
+{
+  var lnrLbl := LearnerHost.InternalLbl();
+  && c.ValidLearnerIdx(lnr)
+  && LearnerHost.Next(c.learnerConstants[lnr], v.Last().learners[lnr], v'.Last().learners[lnr], lnrLbl)
+  && LearnersUnchangedExcept(c, v.Last(), v'.Last(), lnr)
+  && LeadersUnchanged(v.Last(), v'.Last())
+  && AcceptorsUnchanged(v.Last(), v'.Last())
+}
+
+ghost predicate NextStep(c: Constants, v: Variables, v': Variables, step: Step)
+  requires v.WF(c) && v'.WF(c)
+{
+  match step
+    case P1aStep(ldr, acc) => NextP1aStep(c, v, v', ldr, acc)
+    case P1bStep(acc, ldr, balOpt, vbOptOpt) => NextP1bStep(c, v, v', ldr, acc, balOpt, vbOptOpt)
+    case P2aStep(ldr, acc, val) => NextP2aStep(c, v, v', ldr, acc, val)
+    case P2bStep(acc, lnr, vb) => NextP2bStep(c, v, v', acc, lnr, vb)
+    case LearnerInternalStep(lnr) => NextLearnerInternalStep(c, v, v', lnr)
+    case StutterStep => v' == v
+}
+
+ghost predicate Next(c: Constants, v: Variables, v': Variables)
+{
+  && v.WF(c)
+  && v'.WF(c)
+  && exists step :: NextStep(c, v, v', step)
+}
+
+
+//// Helper Functions ////
+
+ghost predicate LeadersUnchanged(h: Hosts, h': Hosts) {
+  h'.leaders == h.leaders
+}
+
+ghost predicate LeadersUnchangedExcept(c: Constants, h: Hosts, h': Hosts, ldr: LeaderId)
+  requires h.WF(c) && h'.WF(c)
+  requires c.ValidLeaderIdx(ldr)
+{
+  forall id:nat | c.ValidLeaderIdx(id) && id != ldr
+  :: h.leaders[id] == h'.leaders[id]
+}
+
+ghost predicate AcceptorsUnchanged(h: Hosts, h': Hosts) {
+  h'.acceptors == h.acceptors
+}
+
+ghost predicate AcceptorsUnchangedExcept(c: Constants, h: Hosts, h': Hosts, acc: AcceptorId)
+  requires h.WF(c) && h'.WF(c)
+  requires c.ValidAcceptorIdx(acc)
+{
+  forall id:nat | c.ValidAcceptorIdx(id) && id != acc
+  :: h.acceptors[id] == h'.acceptors[id]
+}
+
+ghost predicate LearnersUnchanged(h: Hosts, h': Hosts) {
+  h'.learners == h.learners
+}
+
+ghost predicate LearnersUnchangedExcept(c: Constants, h: Hosts, h': Hosts, lnr: LearnerId)
+  requires h.WF(c) && h'.WF(c)
+  requires c.ValidLearnerIdx(lnr)
+{
+  forall id:nat | c.ValidLearnerIdx(id) && id != lnr
+  :: h.learners[id] == h'.learners[id]
+}
+
+
+} // end module System
